proofs/core/IndProp.v
@@ -1,161 +1,6 @@
-Inductive even : nat -> Prop :=
-  | ev0: even 0
-  | evSS: forall n, even n -> even (S (S n)).
-
-Definition even_ind_ty : Prop :=
-forall P : nat -> Prop,
-    P 0 ->
-    (forall n : nat, even n -> P n -> P (S (S n))) ->
-    forall n : nat, even n -> P n.
-
-(*Let's see*)
-Definition test1 : nat -> Prop :=
-  fun m => forall (P: nat -> Prop),
-    P 0 ->
-    (forall n, P n -> P(S (S n))) ->
-    P m.
-
-(*Prove least fixpoint*)
-Lemma least_fp : forall (P: nat -> Prop),
-  P 0 ->
-  (forall n, P n -> P(S (S n))) ->
-  (forall m, test1 m -> P m).
-Proof.
-  intros P H0 Hs m. unfold test1; intros. apply H; auto.
-Qed.
-(*Other direction does not hold (as it shouldn't)*)
-Lemma least_fp' : forall (P: nat -> Prop),
-  P 0 ->
-  (forall n, P n -> P(S (S n))) ->
-  (forall m, P m -> test1 m).
-Proof.
-  intros P H0 Hs m Hp. unfold test1. intros.
-Abort.
-
-Lemma constr_test1: test1 0.
-Proof.
-  unfold test1. intros. apply H.
-Qed.
-
-Lemma constr_test2: forall n, test1 n -> test1 (S (S n)).
-Proof.
-  intros n Hn. unfold test1. intros P Hp0 Hpss.
-  apply Hpss.
-  apply least_fp; assumption.
-Qed.
-
-Lemma see: forall n, even n -> test1 n.
-Proof.
-  intros n He. unfold test1. intros P Hp0 Hps. induction He.
-  auto. subst. apply Hps. auto.
-Qed.
-
-Lemma see2: forall n, test1 n -> even n.
-Proof.
-  intros n. unfold test1. intros Htest.
-  specialize (Htest even). apply Htest; constructor. auto.
-Qed.
-
-Lemma equiv: forall n, even n <-> test1 n.
-Proof.
-  intros n. split. apply see. apply see2.
-Qed.
-
-
-
-(*What if we had something non strictly positive?*)
-Fail Inductive bad : nat -> Prop :=
-  | Bad1: forall n, (bad n -> False) -> bad (S n).
-
-Definition bad1 : nat -> Prop :=
-    fun m => forall (P: nat -> Prop),
-      (forall n, (P n -> False) -> P (S n)) -> P m.
-(*So this is definable - problem is that it isn't really usable?*)
-(*So i think the idea is: if non strictly positive, this Prop may
-not be inhabited - but yeah, where do we need this info?*)
-
-(*Test*)
-Lemma bad1_bad: forall n, (bad1 n -> False) -> bad1 (S n).
-Proof.
-  intros n Hfalse. unfold bad1. intros P Hfalse'.
-  apply Hfalse'.
-  (*Here is where it should fail: it is NOT the case that (~bad1 n) -> ~(P n)*)
-  intros Hp. apply Hfalse. unfold bad1. intros P' Hp'.
-  (*???*)
-  Abort.
-
-Definition odd n := ~(even n).
-Fixpoint evenb (n: nat) : bool :=
-  match n with
-  | O => true
-  | S O => false
-  | S (S n) => evenb n
-  end.
-(*We assume this*)
-Require Import Coq.Arith.Wf_nat.
-Lemma evenb_spec: forall n, even n <-> evenb n = true.
-Proof.
-  intros n.
-  apply  lt_wf_ind with(P:= (fun n => even n <-> evenb n = true)).
-  intros n' IH.
-  destruct n'; simpl; auto; split; intros; auto.
-  constructor.
-  destruct n'. inversion H. inversion H; subst.
-  apply IH; auto. destruct n'. inversion H.
-  constructor. apply IH; auto.
-Qed.
-
-(*2 properties about evenness and oddness*)
-Lemma even_alt: forall n, ~(even n) -> even (S n).
-Proof.
-induction n.
-- intro C. assert (even 0) by constructor. contradiction.
-- intro C. constructor.
-  destruct (evenb n) eqn : He.
-  + apply evenb_spec; auto.
-  + assert (~ even n). {
-    intro C'. apply evenb_spec in C'. rewrite C' in He; inversion He.
-  }
-  specialize (IHn H). contradiction.
-Qed.
-
-Lemma even_alt': forall n, (even n) -> ~(even (S n)).
-Proof.
-  induction n; intros; intro C; inversion C; subst.
-  apply IHn in H1. contradiction.
-Qed.
-
-Lemma odd_alt: forall n, ~(odd n) -> odd (S n).
-Proof.
-  intros n. unfold odd. intros He.
-  apply even_alt'.
-  destruct (evenb n) eqn : Heb.
-  - apply evenb_spec; auto.
-  - assert (~ (even n)). intro C. apply evenb_spec in C.
-    rewrite C in Heb; inversion Heb. contradiction.
-Qed.
-
-(*This shows why we need strict positivity : if we don't have it,
-  the constructors may not be true/inhabited*)
-Lemma bad1_bad: ~(forall n, (bad1 n -> False) -> bad1 (S n)).
-Proof.
-  intros Hc. unfold bad1 in Hc.
-  assert (even 1). {
-    apply Hc.
-    - intros. specialize (H odd).
-      assert (odd 0). { 
-        apply H.
-        apply odd_alt.
-      }
-      unfold odd in H0.
-      apply H0. constructor.
-    - apply even_alt.
-  }
-  inversion H.
-Qed.
-
-
-(*Now let's try*)
+(*Here we give the denotational semantics for inductive
+  predicates and prove that they are the least fixpoint
+  that makes all the constructors true*)
 Require Import Common.
 Require Import Syntax.
 Require Import Types.
@@ -173,23 +18,16 @@ Section IndPropRep.
 Context {sigma: sig} {gamma: context} 
   (gamma_valid: valid_context sigma gamma)
   (pd: pi_dom).
-  (*(i: pre_interp gamma_valid).*)
 
 Variable all_unif: forall m,
   mut_in_ctx m gamma ->
   uniform m.
 
-Lemma valid_ind_pred: forall p p' (tys: list vty) tms,
-  valid_ind_form p (Fpred p' tys tms) ->
-  tys = map vty_var (p_params p) /\
-  length (p_args p) = length tms /\
-  p = p'.
-Proof.
-  intros. inversion H; subst; auto.
-Qed.
-(*See*)
+Section Def.
 
-(*Alternate approach*)
+(*First, define interpretations*)
+
+(*An interpretation where we substitute p with P*)
 
 Definition interp_with_P (pi: pi_funpred gamma_valid pd) (p: predsym) 
   (P: forall srts, 
@@ -208,8 +46,7 @@ Definition interp_with_P (pi: pi_funpred gamma_valid pd) (p: predsym)
     end;
   constrs := constrs gamma_valid pd pi
 |}.
-(*
-Check preds.*)
+
 (*For the list of predsyms, we need to search through the list
   to apply the correct pred. The dependent types make this
   complicated, so we use a separate function*)
@@ -257,7 +94,39 @@ Definition interp_with_Ps (pi: pi_funpred gamma_valid pd)
   constrs := constrs gamma_valid pd pi
 |}.
 
+Lemma find_apply_pred_in (pf: pi_funpred gamma_valid pd)
+  (ps: list predsym)
+  (Ps: hlist
+  (fun p' : predsym =>
+   forall srts : list sort,
+   arg_list (domain (dom_aux pd)) (predsym_sigma_args p' srts) -> bool)
+  ps)
+  (p: predsym)
+  (Hinp: in_bool predsym_eq_dec p ps) :
+  find_apply_pred pf ps Ps p =
+  get_hlist_elt predsym_eq_dec Ps p Hinp.
+Proof.
+  induction ps; simpl.
+  - inversion Hinp.
+  - revert Hinp. simpl. 
+    destruct (predsym_eq_dec p a); subst; auto.
+Qed.
 
+Lemma find_apply_pred_notin (pf: pi_funpred gamma_valid pd)
+(ps: list predsym)
+(Ps: hlist
+(fun p' : predsym =>
+ forall srts : list sort,
+ arg_list (domain (dom_aux pd)) (predsym_sigma_args p' srts) -> bool)
+ps)
+(p: predsym) :
+~ In p ps ->
+find_apply_pred pf ps Ps p = preds gamma_valid pd pf p.
+Proof.
+  induction ps; simpl; auto.
+  intros Hnot. destruct (predsym_eq_dec p a); subst; auto.
+  exfalso. apply Hnot; auto.
+Qed.
 
 Lemma interp_with_Ps_single (pi: pi_funpred gamma_valid pd)
   (p: predsym)
@@ -278,27 +147,19 @@ Proof.
     contradiction.
 Qed.
 
-
-(*Any valuation is equivalent under each interpretation*)
-(*
-Definition interp_P_val pi p P (v: val_ gamma_valid pi):
-  valuation gamma_valid (interp_with_P pi p P).
-apply (Build_valuation gamma_valid _ 
-  (v_typevar _ _ v) 
-  (v_typevar_val _ _ v)).
-apply (v_vars _ _ v).
-Defined.
-
-Definition interp_Ps_val pi p Pi (v: valuation gamma_valid pi):
-  valuation gamma_valid (interp_with_Ps pi p Pi).
-apply (Build_valuation gamma_valid _ 
-  (v_typevar _ _ v) 
-  (v_typevar_val _ _ v)).
-apply (v_vars _ _ v).
-Defined.*)
-
 Definition iter_and (l: list Prop) : Prop :=
   fold_right and True l.
+
+Lemma prove_iter_and (ps: list Prop):
+  (forall x, In x ps -> x) <-> iter_and ps.
+Proof.
+  induction ps; simpl; split; intros; auto.
+  - destruct H0.
+  - split. apply H. left. reflexivity.
+    rewrite <- IHps. intros x Hinx. apply H. right. assumption.
+  - destruct H. destruct H0; subst; auto.
+    apply IHps; auto.
+Qed. 
 
 Fixpoint dep_map {A B: Type} {P: A -> Prop} (f: forall x, P x -> B)
   (l: list A) (Hall: Forall P l) : list B :=
@@ -345,25 +206,6 @@ Proof.
   erewrite IHl. f_equal. apply Hirrel.
 Qed. 
 
-(*TODO: move*)
-(*Given an element in a list and an hlist, get the corresponding element
-  of the hlist*)
-
-Fixpoint get_hlist_elt {A: Type} (eq_dec: forall x y, {x = y} + {x <> y}) 
-  {f: A -> Type} {l: list A}
-  (h: hlist f l) (x: A)
-  (Hinx: in_bool eq_dec x l) : f x :=
-  (match l as l' return in_bool eq_dec x l' -> hlist f l' -> f x with
-  | nil => fun Hin _ => False_rect _ (not_false Hin)
-  | y :: tl => fun Hin h' =>
-    (match (eq_dec x y) as b return b || in_bool eq_dec x tl ->
-      f x with
-    | left Heq => fun _ => ltac:(rewrite Heq; exact (hlist_hd h'))
-    | right Hneq => fun Hin' => 
-      get_hlist_elt eq_dec (hlist_tl h') x Hin'
-    end) Hin
-  end) Hinx h.
-
 (*Since inductive predicates can be mutually recursive, we need
   a list of predsyms and formula lists. This makes the dependent
   types tricky, since we need a (P: forall srts, arg_list srts -> bool)
@@ -375,7 +217,6 @@ Definition indpred_rep (pf: pi_funpred gamma_valid pd)
   (Hform: Forall (Forall (valid_formula sigma)) (map snd indpred)) 
   (p: predsym)
   (Hin: in_bool predsym_eq_dec p (map fst indpred))
-  (*(Hin: In p (map fst indpred))*)
   (srts: list sort)
   (a: arg_list (domain (dom_aux pd)) 
   (predsym_sigma_args p srts)) : bool :=
@@ -403,17 +244,14 @@ Definition indpred_rep (pf: pi_funpred gamma_valid pd)
        -> 
       (*All of this together implies Pi srts a, for the
         i corresponding to p*)
-      (get_hlist_elt predsym_eq_dec Ps p Hin)
-        (*(In_in_bool predsym_eq_dec _ _ Hin))*) srts a)).
+      (get_hlist_elt predsym_eq_dec Ps p Hin) srts a)).
 
-  (*The encoding we want*)
 (*The version for non-mutual-recursion is a lot simpler*)
 Definition indpred_rep_single (pf: pi_funpred gamma_valid pd) 
 (vt: val_typevar) (vv: val_vars pd vt) (p: predsym)
   (fs: list formula) (Hform: Forall (valid_formula sigma) fs) (srts: list sort) 
   (a: arg_list (domain (dom_aux pd)) 
   (predsym_sigma_args p srts)) : bool :=
-  (*TODO: change preds to Prop instead of bool?*)
   all_dec
   (forall (P: forall (srts: list sort), 
     arg_list (domain (dom_aux pd)) 
@@ -422,19 +260,20 @@ Definition indpred_rep_single (pf: pi_funpred gamma_valid pd)
       pd  all_unif vt (interp_with_P pf p P) vv) 
       fs Hform)) -> P srts a).
 
+(*We prove these equivalent in the single case
+  (it makes things easier when we don't need hlists)*)
+
 Definition Forall_single {A: Type} {P: A -> Prop} {x: list A}
   (Hform: Forall P x) :
   Forall (Forall P) [x] :=
   Forall_cons _  Hform (@Forall_nil (list A) (Forall P)).
 
-  (*TODO: rename*)
 Lemma in_triv {A} p (fs: list A): is_true (in_bool predsym_eq_dec p (map fst [(p, fs)])).
 Proof.
   simpl. destruct (predsym_eq_dec); auto.
 Defined.
 
-(*TODO: this is very, very hard to prove.
-  Dependent types are a nightmare*)
+(*Prove equivalence*)
 Lemma indpred_rep_single_equiv (pf: pi_funpred gamma_valid pd) 
 (vt: val_typevar) (vv: val_vars pd vt) (p: predsym)
 (fs: list formula) (Hform: Forall (valid_formula sigma) fs) (srts: list sort) 
@@ -473,130 +312,117 @@ Proof.
     erewrite dep_map_irrel. apply H0.
     intros. apply fmla_rep_irrel.
 Qed.
-  
-(*Prove that this is the least fixpoint*)
-(*TODO: what is the actual definition*)
+
+End Def.
+
+(*Now we prove that [indpred_rep] is the 
+  least predicate that satifies the constructors. *)
 (*We must show the following: 
-  1. When our intepretations inteprets the predicate(s) P 
-    as [indpred_rep], then 
-    all of the constructor reps should imply P(x)
-  2: For all constructors, f, [[f]]_i holds, where i maps
-    each predicate symbol p to [indpred_rep p].
-  The first part is very easy. The second is very hard.*)
+  1. For all constructors, f, [[f]]_i holds, where i maps
+      each predicate symbol p in ps to [indpred_rep ps p].
+  2. Given any other Ps such that the constructors hold
+    under i, where i maps p in ps to (nth i Ps),
+    then (indpred_rep p ps x) -> (nth i Ps x)
+  The second part is very easy. The first is very hard.*)
 
-(*TODO: move to denotational*)
-Lemma fpred_rep (pd': pi_dom) (pf: pi_funpred gamma_valid pd') 
-  (vt: val_typevar) (vv: val_vars pd' vt)
-(p: predsym) (vs: list vty) (args: list term)
-  (Hval: valid_formula sigma (Fpred p vs args)) :
-  formula_rep gamma_valid pd' all_unif vt pf vv (Fpred p vs args) Hval =
-  preds gamma_valid pd' pf p (map (v_subst (v_typevar vt)) vs)
-    (get_arg_list_pred pd' vt p vs args 
-    (term_rep gamma_valid pd' all_unif vt pf vv)
-    (valid_formula_eq eq_refl Hval)).
+(*First, some helpful lemmas*)
+
+
+(*One of the complications is that the [build_indpred]
+  function is difficult to work with. This is a more
+  useful form *)
+  Lemma build_indpred_iff (pf: pi_funpred gamma_valid pd) 
+  (vt: val_typevar) (vv: val_vars pd vt) (ps: list predsym)
+  (Ps: hlist
+  (fun p' : predsym =>
+   forall srts : list sort,
+   arg_list (domain (dom_aux pd)) (predsym_sigma_args p' srts) -> bool)
+  ps)
+  (fs: list (list formula))
+  (Hform: Forall (Forall (valid_formula sigma)) fs):
+  ((fix build_indpred
+    (l : list (list formula))
+    (Hl : Forall (Forall (valid_formula sigma)) l) {struct l} :
+      Prop :=
+    match
+      l as l'
+      return (Forall (Forall (valid_formula sigma)) l' -> Prop)
+    with
+    | [] =>
+        fun _ : Forall (Forall (valid_formula sigma)) [] => True
+    | fs :: ftl =>
+        fun
+          Hall : Forall (Forall (valid_formula sigma))
+                  (fs :: ftl) =>
+        iter_and
+          (map is_true
+            (dep_map
+                (formula_rep gamma_valid pd all_unif vt
+                  (interp_with_Ps pf ps Ps) vv)
+                fs (Forall_inv Hall))) /\
+        build_indpred ftl (Forall_inv_tail Hall)
+    end Hl) fs Hform) <->
+    (forall (f: list formula)
+    (Hallf: Forall (valid_formula sigma) f)
+    (Hinf: In f fs),
+    iter_and
+    (map is_true
+        (dep_map
+          (formula_rep gamma_valid pd all_unif vt
+              (interp_with_Ps pf ps Ps) vv) f Hallf))).
 Proof.
-  reflexivity.
-Qed.
-
-(*Quick test*)
-
-
-(*Will prove:
-  1. For p = f1 | .. fn,
-    all fn's are true
-  2. Suppose that f1 /\ f2 /\ ... fn -> q.
-    Then p -> q*)
-
-Lemma prove_iter_and (ps: list Prop):
-  (forall x, In x ps -> x) <-> iter_and ps.
-Proof.
-  induction ps; simpl; split; intros; auto.
-  - destruct H0.
-  - split. apply H. left. reflexivity.
-    rewrite <- IHps. intros x Hinx. apply H. right. assumption.
-  - destruct H. destruct H0; subst; auto.
-    apply IHps; auto.
-Qed. 
-
-Lemma simpl_all_dec (P: Prop):
-   (all_dec P) <-> P.
-Proof.
-  split; intros;
-  destruct (all_dec P); auto.
-  inversion H.
+  revert Hform.
+  induction fs; simpl; intros; split; intros; auto.
+  - destruct Hinf.
+  - destruct H as [Hhd Htl].
+    destruct Hinf; subst.
+    + erewrite dep_map_irrel. apply Hhd.
+      intros. apply fmla_rep_irrel.
+    + eapply IHfs. apply Htl. auto.
+  - split.
+    + erewrite dep_map_irrel. apply H. left; auto.
+      intros. apply fmla_rep_irrel.
+    + eapply IHfs. intros. apply H. right; auto.
+  Unshelve.
+  inversion Hform; subst. auto.
 Qed.
 
 Scheme Minimality for valid_ind_form Sort Prop.
 
-(*First, we do the proofs for the non-mutually recursive case,
-  since they are simpler and don't involve hlists*)
-  (*TODO: take out common stuff from here*)
-Section Single.
+Section LeastPred.
 
-(*Prove second part first - this is easy*)
-Theorem indpred_least_pred_single (pf: pi_funpred gamma_valid pd) 
+(*We prove the second part (the "least predicate" part)
+  first, since it is easy*)
+Theorem indpred_least_pred (pf: pi_funpred gamma_valid pd) 
   (vt: val_typevar) (vv: val_vars pd vt)
-  (p: predsym) (fs: list formula) (Hform: Forall (valid_formula sigma) fs):
-  forall (P:
+  (ps: list (predsym * list formula))
+  (Hform: Forall (Forall (valid_formula sigma)) (map snd ps)):
+  forall (Ps: hlist
+    (fun p' : predsym =>
     forall srts : list sort,
-    arg_list (domain (dom_aux pd)) 
-      (predsym_sigma_args p srts) ->
-    bool
-  ),  
+    arg_list (domain (dom_aux pd)) (predsym_sigma_args p' srts) -> bool)
+    (map fst ps)),  
   (*If P holds of all of the constructors*)
-  iter_and
-  (map is_true
-     (dep_map
-        (formula_rep gamma_valid pd 
-          all_unif vt (interp_with_P pf p P)  vv) fs Hform)) ->
+  (forall (fs : list formula) (Hform : Forall (valid_formula sigma) fs),
+    In fs (map snd ps) ->
+      iter_and (map is_true (dep_map
+        (formula_rep gamma_valid pd all_unif vt
+        (interp_with_Ps pf (map fst ps) Ps) vv) fs Hform))) ->
 (*Then indpred_rep p fs x -> P x*)  
-  forall (srts : list sort)
-  (a: arg_list (domain (dom_aux pd)) 
+  forall (p: predsym) (Hinp: in_bool predsym_eq_dec p (map fst ps))
+    (srts: list sort) 
+    (a: arg_list (domain (dom_aux pd)) 
     (predsym_sigma_args p srts)),
-    indpred_rep_single pf vt vv p fs Hform srts a -> P srts a.
+    indpred_rep pf vt vv ps Hform p Hinp srts a ->
+    get_hlist_elt predsym_eq_dec Ps p Hinp srts a.
 Proof.
-  intros P Hand srts a. unfold indpred_rep_single.
+  intros Ps Hand p Hinp srts a.
+  unfold indpred_rep.
   rewrite simpl_all_dec. intros.
-  apply H. apply Hand.
+  apply H.
+  rewrite build_indpred_iff.
+  auto.
 Qed.
-
-(*TODO: prove this later, will require strict positivity*)
-(*A key corollary: if any formula is true under the interpretation
-  where p is sent to [indpred_rep_single], then it is true
-  under any interpretation where p is sent to P, for any P
-  which satisfies all of the constructors*)
-  (*
-Lemma indpred_single_implies (pf: pi_funpred gamma_valid pd) 
-(vt: val_typevar) (vv: val_vars pd vt)
-(p: predsym) (fs: list formula) (Hform: Forall (valid_formula sigma) fs):
-  forall (P:
-    forall srts : list sort,
-    arg_list (domain (dom_aux pd)) 
-      (predsym_sigma_args p srts) ->
-    bool
-  ),  
-  (*If P holds of all of the constructors*)
-  iter_and
-  (map is_true
-    (dep_map
-        (formula_rep gamma_valid pd (interp_with_P pf p P) 
-          all_unif vt vv) fs Hform)) ->
-  forall (f: formula) (Hvalf: valid_formula sigma f), 
-    formula_rep gamma_valid pd (interp_with_P pf p 
-      (indpred_rep_single pf vt vv p fs Hform)) all_unif vt vv f Hvalf ->
-    formula_rep gamma_valid pd (interp_with_P pf p P) all_unif vt vv f Hvalf.
-Proof.
-  intros P Hallp.
-  apply formula_ind with (P1:= fun t => 
-    forall (ty: vty) (Hty1: term_has_type sigma t ty),
-    (*TODO: not true - what about if? what about "if"?*)
-    term_rep gamma_valid pd (interp_with_P pf p (indpred_rep_single pf vt vv p fs Hform))
-      all_unif vt vv t ty Hty1 =
-    term_rep gamma_valid pd (interp_with_P pf p P) all_unif vt vv t ty Hty1); auto; simpl; intros.
-  - admit.
-  - admit.
-  -  simpl.
-    *)
 
 (*On the other hand, the first part is hard (showing that [indpred_rep]
   holds of all constructors). Here is an approach to show it:
@@ -604,13 +430,29 @@ Proof.
     have a bunch of forall quantifiers, followed by a bunch
     of let statements, followed by a chain of impliciations
     ending in indpred_rep p fs x for some x
-  2. From this, unfold the definition of indpred_rep
-    and TODO
-    
-  The first step is not easy. We need to define alpha
-  substitution and some quantifier elimination/prenex normal form*)
+  2. From this, unfold the definition of indpred_rep,
+    and we eventually have to prove that, for each of the
+    "and" formulas in the implication, if [[f]] is true
+    when ps map to [indpred_rep ps], then [[f]] is true
+    when ps map to Ps for any Ps. This is true if f is
+    strictly positive, showing why this condition is crucial.
 
-(*First, we define this transformation*)
+  Step 1 requires a lot of steps
+  1. define variable substitution and prove correctness
+  2. define a function to substitute all bound variables
+    to new, unique values (alpha equivalence)
+  3. define a transformation into the (forall _, let _, and f_i -> f)
+    form, and prove that preserves the semantics.
+    Then, prove that this both ends in P srts x for 
+    [valid_ind_forms] and that the [f_i]'s are strictly
+    positive
+  4. Prove the crucial lemma that [[f]]_[ps->indpred_rep ps] ->
+    [[f]]_[ps->Ps] for any Ps if ps occur strictly
+    positively in f
+  5. Prove the main theorem*)
+
+(*We did steps 1 and 2 in Denotational.v (TODO). We start with
+  step 3*)
 
 Definition tup_1 {A B C D: Type} (x: A * B * C * D) :=
   match x with
@@ -629,7 +471,7 @@ Definition tup_4 {A B C D: Type} (x: A * B * C * D) :=
   | (_, _, _, d) => d
   end.
 
-
+(*The decomposition*)
 Fixpoint indpred_decomp (f: formula) : 
   (list vsymbol * list (vsymbol * term) * list formula * formula) :=
   match f with
@@ -648,180 +490,11 @@ Fixpoint indpred_decomp (f: formula) :
 (*Now we prove that for [valid_ind_form] formulas with
   well-formed bound variables, [indpred_decomp] produces
   an equivalent formula when interpreted.*)
-
   Ltac split_all :=
   repeat match goal with
   | H: ?P /\ ?Q |- _ => destruct H
   | |- ?P /\ ?Q => split
   end.
-
-(*Iterated forall - TODO: maybe move to Denotational*)
-Definition fforalls (vs: list vsymbol) (f: formula) : formula :=
-  fold_right (fun x acc => Fquant Tforall x acc) f vs.
-
-Lemma fforalls_valid (vs: list vsymbol) (f: formula) 
-  (Hval: valid_formula sigma f)
-  (Hall: Forall (fun x => valid_type sigma (snd x)) vs) : 
-  valid_formula sigma (fforalls vs f).
-Proof.
-  induction vs; auto. inversion Hall; subst. 
-  simpl. constructor; auto.
-Qed.
-
-Lemma fforalls_valid_inj (vs: list vsymbol) (f: formula)
-  (Hval: valid_formula sigma (fforalls vs f)):
-  valid_formula sigma f /\ Forall (fun x => valid_type sigma (snd x)) vs.
-Proof.
-  induction vs; auto.
-  simpl in Hval. inversion Hval; subst.
-  specialize (IHvs H4). split_all; auto.
-Qed.
-
-(*Substitute in a bunch of values for a bunch of variables,
-  using an hlist to ensure they have the correct type*)
-Fixpoint substi_mult (vt: val_typevar) (vv: @val_vars sigma pd vt) 
-  (vs: list vsymbol)
-  (vals: hlist (fun x =>
-  domain (dom_aux pd) (v_subst (v_typevar vt) x)) (map snd vs)) :
-  val_vars pd vt :=
-  (match vs as l return hlist  
-    (fun x => domain (dom_aux pd) (v_subst (v_typevar vt) x)) 
-    (map snd l) -> val_vars pd vt with
-  | nil => fun _ => vv
-  | x :: tl => fun h' => 
-     (substi_mult vt (substi pd vt vv x (hlist_hd h')) tl (hlist_tl h')) 
-  end) vals.
-  
-(*And we show that we can use this multi-substitution
-  to interpret [fforalls_val]*)
-Lemma fforalls_val (pf: pi_funpred gamma_valid pd)
-  (vt: val_typevar) (vv: val_vars pd vt) 
-  (vs: list vsymbol) (f: formula) 
-  (Hval: valid_formula sigma f)
-  (Hall: Forall (fun x => valid_type sigma (snd x)) vs):
-  formula_rep gamma_valid pd all_unif vt pf vv (fforalls vs f) 
-    (fforalls_valid vs f Hval Hall) =
-    all_dec (forall (h: hlist  (fun x =>
-      domain (dom_aux pd) (v_subst (v_typevar vt) x)) (map snd vs)),
-      formula_rep gamma_valid pd all_unif vt pf
-        (substi_mult vt vv vs h) f Hval).
-Proof.
-  revert vv.
-  generalize dependent (fforalls_valid vs f Hval Hall).
-  induction vs; simpl; intros Hval' vv.
-  - destruct (formula_rep gamma_valid pd all_unif vt pf vv f Hval') eqn : Hrep; 
-    match goal with |- context[ all_dec ?P ] => destruct (all_dec P); auto end; simpl.
-    + exfalso. apply n; intros. erewrite fmla_rep_irrel. apply Hrep.
-    + rewrite <- Hrep. erewrite fmla_rep_irrel. apply i. constructor.
-  - inversion Hall; subst. specialize (IHvs H2).
-    specialize (IHvs (valid_quant_inj (valid_formula_eq eq_refl Hval'))).
-    rewrite fforall_rep. apply all_dec_eq.
-    split; intros Hforall.
-    + intros h. 
-      specialize (Hforall (hlist_hd h)).
-      rewrite IHvs in Hforall.
-      revert Hforall.
-      match goal with |- context[ all_dec ?P ] => destruct (all_dec P); auto end; simpl.
-    + intros d.
-      rewrite IHvs. 
-      match goal with |- context[ all_dec ?P ] => destruct (all_dec P); auto end; simpl.
-      exfalso. apply n; clear n. intros h.
-      specialize (Hforall (HL_cons _ (snd a) (map snd vs) d h)).
-      apply Hforall.
-Qed.
-
-Lemma fforalls_val' (pf: pi_funpred gamma_valid pd)
-  (vt: val_typevar) (vv: val_vars pd vt) 
-  (vs: list vsymbol) (f: formula) 
-  Hval1 Hval2:
-  formula_rep gamma_valid pd all_unif vt pf vv (fforalls vs f) 
-    Hval2 =
-    all_dec (forall (h: hlist  (fun x =>
-      domain (dom_aux pd) (v_subst (v_typevar vt) x)) (map snd vs)),
-      formula_rep gamma_valid pd all_unif vt pf
-        (substi_mult vt vv vs h) f Hval1).
-Proof.
-  assert (A:=Hval2).
-  apply fforalls_valid_inj in A. split_all.
-  rewrite fmla_rep_irrel with(Hval2:=(fforalls_valid vs f Hval1 H0)).
-  apply fforalls_val.
-Qed.
-
-(*Next we give the valuation for an iterated let. This time,
-  we don't need to worry about hlists*)
-Fixpoint substi_multi_let (pf: pi_funpred gamma_valid pd) (vt: val_typevar) (vv: @val_vars sigma pd vt) 
-(vs: list (vsymbol * term)) 
-  (Hall: Forall (fun x => term_has_type sigma (snd x) (snd (fst x))) vs) :
-val_vars pd vt := 
-  match vs as l return
-  Forall (fun x => term_has_type sigma (snd x) (snd (fst x))) l ->
-  val_vars pd vt
-  with
-  | nil => fun _ => vv
-  | (v, t) :: tl => fun Hall =>
-    substi_multi_let pf vt 
-      (substi pd vt vv v 
-        (term_rep gamma_valid pd all_unif vt pf vv t (snd v) 
-      (Forall_inv Hall))) tl (Forall_inv_tail Hall)
-  end Hall.
-
-Definition iter_flet (vs: list (vsymbol * term)) (f: formula) :=
-  fold_right (fun x acc => Flet (snd x) (fst x) acc) f vs.
-
-Lemma iter_flet_valid (vs: list (vsymbol * term)) (f: formula)
-  (Hval: valid_formula sigma f)
-  (Hall: Forall (fun x => term_has_type sigma (snd x) (snd (fst x))) vs) :
-  valid_formula sigma (iter_flet vs f).
-Proof.
-  induction vs; simpl; auto.
-  inversion Hall; subst.
-  constructor; auto.
-Qed.
-
-Lemma iter_flet_valid_inj (vs: list (vsymbol * term)) (f: formula)
-(Hval: valid_formula sigma (iter_flet vs f)):
-(valid_formula sigma f) /\
-(Forall (fun x => term_has_type sigma (snd x) (snd (fst x))) vs).
-Proof.
-  induction vs; simpl in *; auto.
-  inversion Hval; subst. specialize (IHvs H4).
-  split_all; auto.
-Qed.
-
-Lemma iter_flet_val (pf: pi_funpred gamma_valid pd) 
-  (vt: val_typevar) (vv: @val_vars sigma pd vt) 
-  (vs: list (vsymbol * term)) (f: formula)
-  (Hval: valid_formula sigma f)
-  (Hall: Forall (fun x => term_has_type sigma (snd x) (snd (fst x))) vs) :
-  formula_rep gamma_valid pd all_unif vt pf vv (iter_flet vs f) 
-    (iter_flet_valid vs f Hval Hall) =
-  formula_rep gamma_valid pd all_unif vt pf 
-    (substi_multi_let pf vt vv vs Hall) f Hval.
-Proof.
-  generalize dependent (iter_flet_valid vs f Hval Hall).
-  revert vv.
-  induction vs; intros vv Hval'; simpl.
-  - apply fmla_rep_irrel.
-  - rewrite flet_rep. destruct a. simpl.
-    inversion Hall; subst.
-    rewrite (IHvs (Forall_inv_tail Hall)).
-    f_equal.
-    (*Separately, show that substi_multi_let irrelevant
-      in choice of proofs*)
-      clear.
-      erewrite term_rep_irrel. reflexivity.
-Qed.
-
-Definition iter_fand (l: list formula) : formula :=
-    fold_right (fun f acc => Fbinop Tand f acc) Ftrue l.
-
-Lemma iter_fand_valid (l: list formula) 
-  (Hall: Forall (valid_formula sigma) l) :
-  valid_formula sigma (iter_fand l).
-Proof.
-  induction l; simpl; constructor; inversion Hall; subst; auto.
-Qed.
-
 
 
 (*A few results about [indpred_decomp]*)
@@ -878,52 +551,6 @@ Proof.
   - apply (Tconst (ConstInt 0)).
 Qed.
 
-
-(*TODO: move*)
-Lemma wf_quant (q: quant) (v: vsymbol) (f: formula) :
-  fmla_wf (Fquant q v f) ->
-  fmla_wf f.
-Proof.
-  unfold fmla_wf. simpl. intros. split_all.
-  - inversion H; auto.
-  - intros x C. split_all.
-    apply (H0 x).
-    destruct (vsymbol_eq_dec x v); subst; auto.
-    + inversion H; subst. contradiction.
-    + split. apply in_in_remove; auto. right; auto.
-Qed. 
-
-Lemma wf_binop (b: binop) (f1 f2: formula) :
-  fmla_wf (Fbinop b f1 f2) ->
-  fmla_wf f1 /\ fmla_wf f2.
-Proof.
-  unfold fmla_wf. simpl. rewrite NoDup_app_iff.
-  intros. split_all; auto; intros x C; split_all.
-  - apply (H0 x).
-    split_all. apply union_elts. left; auto.
-    apply in_or_app. left; auto.
-  - apply (H0 x).
-    split_all. apply union_elts. right; auto.
-    apply in_or_app. right; auto.
-Qed.
-
-Lemma wf_let (t: term) (v: vsymbol) (f: formula) :
-  fmla_wf (Flet t v f) ->
-  fmla_wf f.
-Proof.
-  unfold fmla_wf. simpl. intros; split_all; auto; 
-  inversion H; subst; auto.
-  - rewrite NoDup_app_iff in H4; apply H4.
-  - intros x C. split_all.
-    apply (H0 x). split.
-    + apply union_elts. right.
-      apply in_in_remove; auto. intro Heq; subst.
-      inversion H; subst.
-      apply H7. apply in_or_app. right; auto.
-    + right. apply in_or_app. right; auto.
-Qed.
-
-
 Lemma indpred_decomp_wf (f: formula) (Hwf: fmla_wf f):
   (forall x, ~ (In x (tup_1 (indpred_decomp f)) /\ 
     In x (map fst (tup_2 (indpred_decomp f))))).
@@ -974,248 +601,6 @@ Proof.
   apply iter_fand_valid; auto.
   apply indpred_decomp_valid; auto.
 Qed.
-
-Lemma bool_of_binop_impl: forall b1 b2,
-  bool_of_binop Timplies b1 b2 = all_dec (b1 -> b2).
-Proof.
-  intros. destruct b1; destruct b2; simpl;
-  match goal with |- context[ all_dec ?P ] => destruct (all_dec P); auto end;
-  exfalso; apply n; auto.
-Qed.
-
-(*TODO: move*)
-Lemma distr_impl_forall (pf: pi_funpred gamma_valid pd) 
-(vt: val_typevar) (vv: @val_vars sigma pd vt)  
-(f1 f2: formula) (x: vsymbol)
-(Hval1: valid_formula sigma (Fbinop Timplies f1 (Fquant Tforall x f2)))
-(Hval2: valid_formula sigma (Fquant Tforall x (Fbinop Timplies f1 f2))):
-~In x (form_fv f1) ->
-formula_rep gamma_valid pd all_unif vt pf vv
-  (Fbinop Timplies f1 (Fquant Tforall x f2)) Hval1 =
-formula_rep gamma_valid pd all_unif vt pf vv
-  (Fquant Tforall x (Fbinop Timplies f1 f2)) Hval2.
-Proof.
-  intros Hnotin.
-  rewrite fforall_rep, fbinop_rep, bool_of_binop_impl.
-  apply all_dec_eq. rewrite fforall_rep. split; intros.
-  - rewrite fbinop_rep, bool_of_binop_impl, simpl_all_dec.
-    intros.
-    assert (formula_rep gamma_valid pd all_unif vt pf vv f1
-    (proj1 (valid_binop_inj (valid_formula_eq eq_refl Hval1)))). {
-      erewrite form_fv_agree. erewrite fmla_rep_irrel. apply H0.
-      intros. unfold substi.
-      destruct (vsymbol_eq_dec x0 x); subst; auto. contradiction.
-    }
-    specialize (H H1).
-    rewrite simpl_all_dec in H.
-    specialize (H d).
-    erewrite fmla_rep_irrel. apply H.
-  - rewrite simpl_all_dec. intros d.
-    specialize (H d).
-    revert H. rewrite fbinop_rep, bool_of_binop_impl, simpl_all_dec;
-    intros.
-    erewrite fmla_rep_irrel.
-    apply H. erewrite form_fv_agree. erewrite fmla_rep_irrel. apply H0.
-    intros. unfold substi. destruct (vsymbol_eq_dec x0 x); subst; auto.
-    contradiction.
-Qed.
-
-(*TODO: move*)
-Lemma distr_impl_let (pf: pi_funpred gamma_valid pd) 
-(vt: val_typevar) (vv: @val_vars sigma pd vt)  
-(f1 f2: formula) (t: term) (x: vsymbol)
-(Hval1: valid_formula sigma (Fbinop Timplies f1 (Flet t x f2)))
-(Hval2: valid_formula sigma (Flet t x (Fbinop Timplies f1 f2))):
-~In x (form_fv f1) ->
-formula_rep gamma_valid pd all_unif vt pf vv
-  (Fbinop Timplies f1 (Flet t x f2)) Hval1 =
-formula_rep gamma_valid pd all_unif vt pf vv
-  (Flet t x (Fbinop Timplies f1 f2)) Hval2.
-Proof.
-  intros.
-  rewrite flet_rep, !fbinop_rep, !bool_of_binop_impl.
-  apply all_dec_eq.
-  rewrite flet_rep.
-  erewrite form_fv_agree.
-  erewrite (form_fv_agree _ _ _ _ _ f2).
-  erewrite fmla_rep_irrel.
-  erewrite (fmla_rep_irrel _ _ _ _ _ _ f2).
-  reflexivity.
-  all: intros; unfold substi;
-  destruct (vsymbol_eq_dec x0 x); subst; auto; try contradiction.
-  unfold eq_rec_r, eq_rec, eq_rect. simpl.
-  apply term_rep_irrel.
-Qed.
-  
-
-(*TODO: move*)
-(*If the formula is wf, we can move an implication
-  across lets and foralls *)
-(*NOTE: know no overlap because all vars in quants and lets
-  come from f2 - must be bound vars in f2 (TODO: prove)
-  so this is safe*)
-Lemma distr_impl_let_forall (pf: pi_funpred gamma_valid pd) 
-  (vt: val_typevar) (vv: @val_vars sigma pd vt)  
-  (f1 f2: formula)
-  (q: list vsymbol) (l: list (vsymbol * term))
-  (Hval1: valid_formula sigma (fforalls q (iter_flet l (Fbinop Timplies f1 f2))))
-  (Hval2: valid_formula sigma (Fbinop Timplies f1 (fforalls q (iter_flet l f2))))
-  (Hq: forall x, ~ (In x q /\ In x (form_fv f1)))
-  (Hl: forall x, ~ (In x l /\ In (fst x) (form_fv f1))) :
-  formula_rep gamma_valid pd all_unif vt pf vv
-    (fforalls q (iter_flet l (Fbinop Timplies f1 f2))) Hval1 =
-  formula_rep gamma_valid pd all_unif vt pf vv
-    (Fbinop Timplies f1 (fforalls q (iter_flet l f2))) Hval2.
-Proof.
-  revert vv.
-  induction q.
-  - simpl.
-    (*Prove let case here*)
-    induction l; simpl; auto.
-    + intros. apply fmla_rep_irrel.
-    + intros. erewrite distr_impl_let.
-      * erewrite !flet_rep, IHl.
-        f_equal. f_equal. apply term_rep_irrel.
-        intros x C. apply (Hl x). split_all; auto. right; auto.
-        (*Go back and do [valid_formula]*)
-        Unshelve.
-        simpl in Hval1. simpl in Hval2.
-        inversion Hval1; subst.
-        constructor; auto.
-        inversion Hval2; subst.
-        constructor; auto.
-        inversion H6; subst; auto.
-      * intro C. apply (Hl a). split_all; auto. left; auto.
-  - intros vv. simpl.
-    erewrite distr_impl_forall.
-    + rewrite !fforall_rep. apply all_dec_eq.
-      split; intros.
-      * erewrite  <- IHq. apply H.
-        intros. intro C. apply (Hq x). split_all; auto.
-        right; auto.
-      * erewrite IHq. apply H. intros. intro C. apply (Hq x).
-        split_all; auto. right; auto.
-        (*Go back and do [valid_formula]*)
-        Unshelve.
-        simpl in Hval1; simpl in Hval2; inversion Hval1; 
-        inversion Hval2; subst.
-        constructor; auto. constructor; auto.
-        inversion H10; subst. auto.
-    + intro C.
-      apply (Hq a). split; auto. left; auto.
-Qed.
-
-(*Kind of a silly lemma, but we need to be able
-  to rewrite the first of an implication without
-  unfolding all bound variables
-  *)
-(*TODO: move*)
-Lemma and_impl_bound (pf: pi_funpred gamma_valid pd) 
-(vt: val_typevar) (vv: @val_vars sigma pd vt)  
-(f1 f2 f3: formula)
-(q: list vsymbol) (l: list (vsymbol * term))
-Hval1 Hval2: 
-formula_rep gamma_valid pd all_unif vt pf vv
-  (fforalls q (iter_flet l (Fbinop Timplies (Fbinop Tand f1 f2) f3))) Hval1 =
-formula_rep gamma_valid pd all_unif vt pf vv
-  (fforalls q (iter_flet l (Fbinop Timplies f1 (Fbinop Timplies f2 f3)))) Hval2.
-Proof.
-  assert (A:=Hval1).
-  assert (B:=Hval2).
-  apply fforalls_valid_inj in A.
-  apply fforalls_valid_inj in B. split_all.
-  rewrite (fforalls_val') with(Hval1:=H1).
-  rewrite (fforalls_val') with(Hval1:=H).
-  assert (A:=H1).
-  apply iter_flet_valid_inj in A.
-  assert (B:=H).
-  apply iter_flet_valid_inj in B.
-  split_all.
-  apply all_dec_eq. split; intros Hrep h.
-  - specialize (Hrep h).
-    rewrite fmla_rep_irrel with (Hval1:=H) 
-      (Hval2:=iter_flet_valid  l _ H3 H4).
-    rewrite fmla_rep_irrel with (Hval1:=H1)
-      (Hval2:=iter_flet_valid l _ H5 H4) in Hrep.
-    revert Hrep. rewrite !iter_flet_val.
-    rewrite and_impl with(Hval2:=H3).
-    intros C; apply C.
-  - specialize (Hrep h).
-    rewrite fmla_rep_irrel with (Hval1:=H) 
-      (Hval2:=iter_flet_valid  l _ H3 H4) in Hrep.
-    rewrite fmla_rep_irrel with (Hval1:=H1)
-      (Hval2:=iter_flet_valid l _ H5 H4).
-    revert Hrep. rewrite !iter_flet_val.
-    rewrite and_impl with(Hval2:=H3).
-    intros C; apply C.
-Qed.
-
-(*Last (I hope) intermediate lemma: we can
-  push a let outside of foralls if the variable does not
-  appear quantified and no free variables in the term appear in
-  the list either*)
-Lemma distr_let_foralls (pf: pi_funpred gamma_valid pd) 
-(vt: val_typevar) (vv: @val_vars sigma pd vt)  
-(t: term) (x: vsymbol) (f: formula)
-(q: list vsymbol) Hval1 Hval2:
-(~ In x q) ->
-(forall y, In y (term_fv t) -> ~ In y q) ->
-formula_rep gamma_valid pd all_unif vt pf vv
-  (fforalls q (Flet t x f)) Hval1 =
-formula_rep gamma_valid pd all_unif vt pf vv
-  (Flet t x (fforalls q f)) Hval2.
-Proof.
-  intros. revert vv. induction q; intros vv.
-  - simpl. apply fmla_rep_irrel.
-  - simpl. (*Here, we prove the single transformation*)
-    rewrite fforall_rep, flet_rep, fforall_rep.
-    assert (Hval3: valid_formula sigma (Flet t x (fforalls q f))). {
-        simpl in Hval2. inversion Hval2; subst.
-        inversion H6; subst. constructor; auto.
-      }
-    assert (Hnotx: ~ In x q). {
-      intro C. apply H. right; auto.
-    }
-    assert (Hinq: forall y : vsymbol, In y (term_fv t) -> ~ In y q). {
-      intros y Hy C. apply (H0 y); auto. right; auto.
-    }
-    apply all_dec_eq. split; intros Hrep d; specialize (Hrep d).
-    + rewrite IHq with (Hval2:=Hval3) in Hrep; auto.
-      rewrite flet_rep in Hrep.
-      rewrite substi_diff.
-      rewrite term_rep_irrel with(Hty2:=(proj1 (valid_let_inj (valid_formula_eq eq_refl Hval3)))).
-      rewrite fmla_rep_irrel with (Hval2:=(proj2 (valid_let_inj (valid_formula_eq eq_refl Hval3)))).
-      erewrite term_fv_agree in Hrep. apply Hrep.
-      intros. unfold substi. destruct (vsymbol_eq_dec x0 a); subst; auto.
-      exfalso. apply (H0 a); auto. left; auto.
-      intro; subst. apply H. left; auto.
-    + rewrite IHq with (Hval2:=Hval3); auto.
-      rewrite flet_rep.
-      rewrite substi_diff.
-      rewrite term_rep_irrel with(Hty2:=(proj1 (valid_let_inj (valid_formula_eq eq_refl Hval2)))).
-      rewrite fmla_rep_irrel with (Hval2:=(valid_quant_inj
-      (valid_formula_eq eq_refl
-         (proj2 (valid_let_inj (valid_formula_eq eq_refl Hval2)))))).
-      erewrite term_fv_agree in Hrep. apply Hrep.
-      intros. unfold substi. destruct (vsymbol_eq_dec x0 a); subst; auto.
-      exfalso. apply (H0 a); auto. left; auto.
-      intro; subst. apply H. left; auto.
-Qed.
-
-
-      (*Now need to simplify let and generalize v*)
-      (*TODO: start here - should be doable, just need to push through*)
-(*After, finish following lemma, equal interp
-  THEN prove that for valid_ind_form, last is p tys tms for tys and
-  tms we can get in a function
-  THEN prove (probably) that this is still strictly positive
-  THEN try to prove main theorem, see where we get stuck
-  and see if assuming SP -> (indpred -> P) lets us prove it
-  if so, go back to that lemma and prove
-  finally, deal with alpha substitution (can assume as
-    axiom for now)
-  also fix those admitted cases in denot
-  *)
 
 (*Now, we prove that any formula which is valid and whose bound
   variables are well-formed is equivalent to the one formed
@@ -1292,7 +677,7 @@ Proof.
       apply iter_flet_valid_inj in H2; split_all.
       inversion H2; subst. constructor; auto. 
     }
-    rewrite (distr_impl_let_forall _ _ _ f1) with(Hval2:=Hval3).
+    rewrite (distr_impl_let_forall _ _ _ vt pf vv f1) with(Hval2:=Hval3).
     + rewrite fbinop_rep, bool_of_binop_impl.
       apply all_dec_eq. split; intros;
       erewrite fmla_rep_irrel;
@@ -1373,7 +758,7 @@ Proof.
 Qed.
 
 (** Results based on Positivity/Strict Positivity *)
-(*TODO: move maybe*)
+
 Lemma positive_fforalls (ps: list predsym) (q: list vsymbol) (f: formula):
   ind_positive ps f <->
   ind_positive ps (fforalls q f).
@@ -1382,14 +767,6 @@ Proof.
   - induction q; intros; simpl; auto. constructor; auto.
   - induction q; simpl; auto; intros. inversion H; subst; auto.
 Qed.
-(*
-Lemma positive_fforalls (ps: list predsym) (q: list vsymbol) (f: formula):
-  ind_positive ps (fforalls q f) ->
-  ind_positive ps f.
-Proof.
-  induction q; simpl; auto. intros.
-  inversion H; subst. auto.
-Qed.*)
 
 Lemma positive_iter_flet (ps: list predsym) (l: list (vsymbol * term))
   (f: formula):
@@ -1426,7 +803,6 @@ Proof.
     apply ISP_and; auto.
 Qed.
 
-(*TODO: move*)
 Lemma strict_pos_and (ps: list predsym) (f1 f2: formula):
   ind_strictly_positive ps (Fbinop Tand f1 f2) ->
   ind_strictly_positive ps f1 /\
@@ -1518,66 +894,6 @@ Proof.
   apply fmla_closed_val; auto.
 Qed.
 
-
-(*One of the complications is that the [build_indpred]
-  function is difficult to work with *)
-
-Lemma build_indpred_iff (pf: pi_funpred gamma_valid pd) 
-  (vt: val_typevar) (vv: val_vars pd vt) (ps: list predsym)
-  (Ps: hlist
-  (fun p' : predsym =>
-   forall srts : list sort,
-   arg_list (domain (dom_aux pd)) (predsym_sigma_args p' srts) -> bool)
-  ps)
-  (fs: list (list formula))
-  (Hform: Forall (Forall (valid_formula sigma)) fs):
-  ((fix build_indpred
-    (l : list (list formula))
-    (Hl : Forall (Forall (valid_formula sigma)) l) {struct l} :
-      Prop :=
-    match
-      l as l'
-      return (Forall (Forall (valid_formula sigma)) l' -> Prop)
-    with
-    | [] =>
-        fun _ : Forall (Forall (valid_formula sigma)) [] => True
-    | fs :: ftl =>
-        fun
-          Hall : Forall (Forall (valid_formula sigma))
-                  (fs :: ftl) =>
-        iter_and
-          (map is_true
-            (dep_map
-                (formula_rep gamma_valid pd all_unif vt
-                  (interp_with_Ps pf ps Ps) vv)
-                fs (Forall_inv Hall))) /\
-        build_indpred ftl (Forall_inv_tail Hall)
-    end Hl) fs Hform) <->
-    (forall (f: list formula)
-    (Hallf: Forall (valid_formula sigma) f)
-    (Hinf: In f fs),
-    iter_and
-    (map is_true
-        (dep_map
-          (formula_rep gamma_valid pd all_unif vt
-              (interp_with_Ps pf ps Ps) vv) f Hallf))).
-Proof.
-  revert Hform.
-  induction fs; simpl; intros; split; intros; auto.
-  - destruct Hinf.
-  - destruct H as [Hhd Htl].
-    destruct Hinf; subst.
-    + erewrite dep_map_irrel. apply Hhd.
-      intros. apply fmla_rep_irrel.
-    + eapply IHfs. apply Htl. auto.
-  - split.
-    + erewrite dep_map_irrel. apply H. left; auto.
-      intros. apply fmla_rep_irrel.
-    + eapply IHfs. intros. apply H. right; auto.
-  Unshelve.
-  inversion Hform; subst. auto.
-Qed.
-
 Lemma indpred_rep_val_eq (pf: pi_funpred gamma_valid pd)
   (vt: val_typevar) (v1 v2: val_vars pd vt)
   (ps: list (predsym * list formula))
@@ -1598,491 +914,36 @@ Proof.
   rewrite Forall_forall in Hclosed; apply Hclosed; assumption.
 Qed.
 
-Lemma indpred_rep_single_val_eq (pf: pi_funpred gamma_valid pd)
-(vt: val_typevar) (v1 v2: val_vars pd vt) (p: predsym)
-(fs: list formula) 
-(Hform: Forall (valid_formula sigma) fs)
-(Hclosed: Forall closed_formula fs) :
-  indpred_rep_single pf vt v1 p fs Hform =
-  indpred_rep_single pf vt v2 p fs Hform.
-Proof.
-  unfold indpred_rep_single. 
-  repeat(apply functional_extensionality_dep; intros).
-  apply all_dec_eq.
-  split; intros Hand P; specialize (Hand P);
-  erewrite constrs_val_eq; auto; apply Hand.
-Qed.
-
-(*Let us prove the following: for a closed formula, the interpretation
-  is equivalent under any valuation. Basically, we want to prove
-  that [indpred_rep_single], as well as the [formula_rep]s for the
-  constructors, can be evaluated under any valuation with the same
-  results*)
 (*Now we prove our key intermediate lemma that we need:
   suppose f is a formula in which p appears strictly positiviely,
   then [[f]]_(p->indpred_rep p) implies [[f]]_(p->P) for any P*)
-Lemma strict_pos_impred_implies_P (pf: pi_funpred gamma_valid pd) 
-(vt: val_typevar) (vv: val_vars pd vt)
-(p: predsym) (ps: list predsym) 
-(fs: list formula) 
-(Hinp: In p ps)
-(f: formula)
-(Hvalf: valid_formula sigma f)
-(Hpos: ind_strictly_positive ps f)
-(Hform: Forall (valid_formula sigma) fs)
-(Hclosed: Forall closed_formula fs)
-(Hindpred: preds gamma_valid pd pf p = indpred_rep_single pf vt vv p fs Hform)
-:
-forall (P: forall srts : list sort,
-  arg_list (domain (dom_aux pd)) (predsym_sigma_args p srts) ->
-  bool),  
-(*If P holds of all of the constructors*)
-iter_and (map is_true (dep_map
-  (formula_rep gamma_valid pd all_unif vt 
-    (interp_with_P pf p P) vv) fs Hform)) ->
-(*Then [[f]]_(p->indpred_rep p) implies [[f]]_(p->P)*) 
-formula_rep gamma_valid pd all_unif vt pf vv f Hvalf ->
-formula_rep gamma_valid pd all_unif vt (interp_with_P pf p P) vv f Hvalf.
-Proof.
-  intros P HandP.
-  generalize dependent vv.
-  induction Hpos; simpl; intros vv Hindpred HandP; auto.
-  - intros Hrep. erewrite fmla_predsym_agree. apply Hrep.
-    all: auto.
-    intros p' Hinp'.
-    unfold interp_with_P; simpl.
-    destruct (predsym_eq_dec p p'); subst; auto.
-    specialize (H p' Hinp). rewrite Hinp' in H. inversion H.
-  - rewrite !fpred_rep. simpl.
-    (*Show arg lists are the same: because P cannot appear
-      in list by strict positivity*)
-    assert ((get_arg_list_pred pd vt p0 vs ts
-    (term_rep gamma_valid pd all_unif vt pf vv)
-    (valid_formula_eq eq_refl Hvalf)) =  (get_arg_list_pred pd vt p0 vs ts
-    (term_rep gamma_valid pd all_unif vt (interp_with_P pf p P) vv)
-    (valid_formula_eq eq_refl Hvalf))). {
-      apply get_arg_list_pred_eq.
-      rewrite Forall_forall. intros.
-      rewrite term_rep_irrel with(Hty2:=Hty2).
-      apply term_predsym_agree; simpl; auto.
-      intros p' Hinp'.
-      destruct (predsym_eq_dec p p'); subst; auto; simpl.
-      specialize (H0 _ _ H1 Hinp).
-      rewrite Hinp' in H0. inversion H0.
-    }
-    destruct (predsym_eq_dec p p0); subst; simpl; auto.
-    + rewrite Hindpred, H1.
-      apply indpred_least_pred_single with(P:=P); auto. 
-    + rewrite H1. auto.
-  - rewrite !fbinop_rep, !bool_of_binop_impl, !simpl_all_dec.
-    intros Hinpl Hval.
-    apply IHHpos; auto.
-    apply Hinpl. 
-    (*Now we use the fact that P is not in f1*)
-    rewrite (fmla_predsym_agree) with(p2:=(interp_with_P pf p P)); auto.
-    intros p' Hinp'.
-    simpl. destruct (predsym_eq_dec p p'); subst; auto.
-    specialize (H _ Hinp). rewrite Hinp' in H. inversion H.
-  - destruct q.
-    + rewrite !fforall_rep, !simpl_all_dec; intros Hall d; specialize (Hall d).
-      apply IHHpos; auto.
-      (*Use closed fmla assumptions*)
-      erewrite indpred_rep_single_val_eq; auto. apply Hindpred.
-      erewrite constrs_val_eq; auto. apply HandP.
-    + rewrite !fexists_rep, !simpl_all_dec; intros [d Hex]; exists d.
-      apply IHHpos; auto.
-      erewrite indpred_rep_single_val_eq; auto. apply Hindpred.
-      erewrite constrs_val_eq; auto. apply HandP.
-  - rewrite !fbinop_rep; simpl; unfold is_true; rewrite !andb_true_iff;
-    intros [Hf1 Hf2].
-    split; [apply IHHpos1 | apply IHHpos2]; auto.
-  - rewrite !fbinop_rep; simpl; unfold is_true; rewrite !orb_true_iff;
-    intros [Hf1 | Hf2]; 
-    [left; apply IHHpos1 | right; apply IHHpos2]; auto.
-  - rewrite !flet_rep; intros Hf.
-    apply IHHpos; auto. 
-    + erewrite indpred_rep_single_val_eq; auto. apply Hindpred.
-    + erewrite constrs_val_eq; auto. apply HandP.
-    + (*Need fact that p doesn't appear in let term*)
-      erewrite term_predsym_agree. apply Hf. all: auto.
-      intros p' Hinp'. unfold interp_with_P; simpl.
-      destruct (predsym_eq_dec p p'); subst; auto.
-      specialize (H _ Hinp). rewrite Hinp' in H. inversion H.
-  - rewrite !fif_rep.
-    (*First, know that [[f1]] eq in both cases because P cannot be
-      present*)
-    assert (Hf1: formula_rep gamma_valid pd all_unif vt pf vv f1
-    (proj1 (valid_if_inj (valid_formula_eq eq_refl Hvalf))) =
-    formula_rep gamma_valid pd all_unif vt (interp_with_P pf p P) vv f1
-    (proj1 (valid_if_inj (valid_formula_eq eq_refl Hvalf)))). {
-      apply fmla_predsym_agree; auto; simpl; intros p' Hinp'.
-      destruct (predsym_eq_dec p p'); subst; auto.
-      specialize (H _ Hinp). rewrite Hinp' in H; inversion H.
-    }
-    rewrite <- Hf1.
-    destruct (formula_rep gamma_valid pd all_unif vt pf vv f1
-    (proj1 (valid_if_inj (valid_formula_eq eq_refl Hvalf))));
-    [apply IHHpos1 | apply IHHpos2]; auto.
-  - (*Hmm, this is the hardest one - need rewrite lemma for match*)
-    rewrite !fmatch_rep.
-    (*Here, we need a nested induction*)
-    generalize dependent (proj2 (valid_match_inv (valid_formula_eq eq_refl Hvalf))).
-    generalize dependent  (proj1 (valid_match_inv (valid_formula_eq eq_refl Hvalf))).
-    clear Hvalf.
-    induction pats; simpl; auto.
-    intros Hty Hallval. destruct a as [fh ph].
-    (*Show that [term_rep] is equal because P cannot appear*)
-    assert (Hteq: 
-    (term_rep gamma_valid pd all_unif vt pf vv t ty Hty) =
-    (term_rep gamma_valid pd all_unif vt (interp_with_P pf p P) vv t ty Hty)). {
-      apply term_predsym_agree; auto. intros p' Hinp'; simpl.
-      destruct (predsym_eq_dec p p'); subst; auto.
-      specialize (H _ Hinp). rewrite Hinp' in H. inversion H.
-    }
-    rewrite <- Hteq at 1.
-    destruct (match_val_single gamma_valid pd all_unif vt ty
-    (has_type_valid gamma_valid t ty Hty)
-    (term_rep gamma_valid pd all_unif vt pf vv t ty Hty) fh) eqn : Hm.
-    + (*First case follows from original IH*) 
-      apply H1; simpl; auto.
-      * erewrite indpred_rep_single_val_eq; auto. apply Hindpred.
-      * erewrite constrs_val_eq; auto. apply HandP.
-    + (*From nested IH*)
-      apply IHpats; auto.
-      * intros h Hinf. apply H0. right; auto.
-      * intros. apply H1; auto. right; auto.
-Qed.
-
-(*We axiomatize alpha substitution, we will do it later*)
-Axiom alpha_f : formula -> formula.
-
-Axiom alpha_valid : forall (f: formula) (Hval: valid_formula sigma f),
-  valid_formula sigma (alpha_f f).
-
-Axiom alpha_f_equiv : forall (pf: pi_funpred gamma_valid pd)
-  (vt: val_typevar) (vv: val_vars pd vt) 
-  (f: formula) (Hvalf: valid_formula sigma f),
-  formula_rep gamma_valid pd all_unif vt pf vv f Hvalf =
-  formula_rep gamma_valid pd all_unif vt pf vv (alpha_f f) 
-    (alpha_valid f Hvalf).
-
-Axiom alpha_f_wf: forall (f: formula), fmla_wf (alpha_f f).
-
-Axiom alpha_valid_ind_form: forall (p: predsym) (f: formula),
-  valid_ind_form p f ->
-  valid_ind_form p (alpha_f f).
-
-Axiom alpha_pos: forall (ps: list predsym) (f: formula),
-  ind_positive ps f ->
-  ind_positive ps (alpha_f f).
-
-(*TODO: move*)
-(*If some pred P does not appear in any terms for [substi_multi_let],
-  then valuations are equal no matter what P is*)
-
-Lemma substi_mult_notin_eq (pf1 pf2: pi_funpred gamma_valid pd) 
-  (vt: val_typevar) (vv: val_vars pd vt) (l: list (vsymbol * term))
-  (ps: list predsym) Hall
-  (Hallnotin: Forall (fun x => (forall p, In p ps -> 
-    negb (predsym_in_term p (snd x)))) l) :
-  (forall p, ~ In p ps -> (preds gamma_valid pd pf1 p) = (preds gamma_valid pd pf2 p)) ->
-  (forall f, funs gamma_valid pd pf1 f = funs gamma_valid pd pf2 f) ->
-  substi_multi_let pf1 vt vv l Hall =
-  substi_multi_let pf2 vt vv l Hall.
-Proof.
-  revert Hall vv.
-  induction l; simpl; auto; intros.
-  inversion Hallnotin; subst.
-  destruct a.
-  assert (substi pd vt vv v
-  (term_rep gamma_valid pd all_unif vt pf1 vv t (snd v) (Forall_inv Hall)) =
-  (substi pd vt vv v
-     (term_rep gamma_valid pd all_unif vt pf2 vv t (snd v) (Forall_inv Hall)))). {
-    unfold substi. apply functional_extensionality_dep; intros; simpl.
-    destruct (vsymbol_eq_dec x v); subst; auto.
-    unfold eq_rec_r, eq_rec, eq_rect. simpl.
-    apply term_predsym_agree; auto.
-    intros p Hinp.
-    apply H. intro Hinp'.
-    simpl in H3. apply H3 in Hinp'.
-    rewrite Hinp in Hinp'. inversion Hinp'.
-  }
-  rewrite H1.
-  apply IHl; auto.
-Qed.
-
-(*TODO: move*)
-Lemma iter_fand_rep (pd': pi_dom) (pf: pi_funpred gamma_valid pd') 
-(vt: val_typevar) (vv: val_vars pd' vt) 
-(l: list formula)
-(Hall: valid_formula sigma (iter_fand l)) :
-formula_rep gamma_valid pd' all_unif vt pf vv (iter_fand l) Hall <->
-(forall (f: formula) (Hvalf: valid_formula sigma f),
-  In f l -> formula_rep gamma_valid pd' all_unif vt pf vv f Hvalf).
-Proof.
-  revert Hall.
-  induction l; simpl; intros; auto; split; intros; auto.
-  - rewrite fbinop_rep in H.
-    simpl in H. unfold is_true in H. rewrite andb_true_iff in H.
-    destruct H.
-    destruct H0; subst.
-    + erewrite fmla_rep_irrel. apply H.
-    + inversion Hall; subst.
-      specialize (IHl H7).
-      apply IHl; auto.
-      erewrite fmla_rep_irrel. apply H1.
-  - rewrite fbinop_rep. simpl.
-    inversion Hall; subst.
-    specialize (IHl H5).
-    apply andb_true_iff. split.
-    + erewrite fmla_rep_irrel. apply H. left; auto.
-    + erewrite fmla_rep_irrel. apply IHl. intros.
-      apply H. right; auto.
-      Unshelve.
-      auto.
-Qed.
-
-(*Now we (at least state) the main theorem*)
-(*This is the non-mutual version, mutual should be similar*)
-(*TODO: will need to show that [indpred_rep_single] is
-  equal on all valuations even if their values for (preds p) 
-  are different (not hard)*)
-Theorem indpred_constrs_true
-  (pf: pi_funpred gamma_valid pd)
+Lemma strict_pos_impred_implies_P' (pf: pi_funpred gamma_valid pd) 
   (vt: val_typevar) (vv: val_vars pd vt)
-  (p: predsym) (fs: list formula)
-  (Hform: Forall (valid_formula sigma) fs)
-  (Hvalind: Forall (fun f => valid_ind_form p f) fs)
-  (Hpos: Forall (fun f => ind_positive [p] f) fs)
-  (Hclosed: Forall closed_formula fs)
-  (Hindpred: (preds gamma_valid pd pf) p = 
-    indpred_rep_single pf vt vv p fs Hform) :
-  (forall (f: formula) (Hvalf: valid_formula sigma f), 
-    In f fs ->
-    formula_rep gamma_valid pd all_unif vt pf vv f Hvalf).
-Proof.
-  intros f Hvalf Hinf.
-  (*Part 1: work with alpha to get wf*)
-  rewrite alpha_f_equiv.
-  assert (Hvalindf: valid_ind_form p f). rewrite Forall_forall in Hvalind.
-    apply Hvalind; auto.
-  assert (Hposf: ind_positive [p] f). rewrite Forall_forall in Hpos.
-    apply Hpos; auto.
-  assert (Hvalinda:=(alpha_valid_ind_form p f Hvalindf)).
-  assert (Hwfa:=(alpha_f_wf f)).
-  assert (Hposa:=(alpha_pos [p] f Hposf)).
-  (*Part 2: Work with [indpred_transform] *)
-  rewrite indpred_decomp_equiv; auto.
-  assert (Hvaldec:=(indpred_transform_valid _ (alpha_valid _ Hvalf))).
-  (*Then we can unfold manually*)
-  unfold indpred_transform in *.
-  assert (A:=Hvaldec).
-  apply fforalls_valid_inj in A.
-  destruct A as [Hval1 Halltup1].
-  rewrite fmla_rep_irrel with
-    (Hval2:= (fforalls_valid (tup_1 (indpred_decomp (alpha_f f))) _ Hval1 Halltup1)).
-  rewrite fforalls_val. rewrite simpl_all_dec. intros h.
-  assert (A:=Hval1).
-  apply iter_flet_valid_inj in A.
-  destruct A as [Hval2 Halltup2].
-  rewrite (fmla_rep_irrel) with(Hval2:=(iter_flet_valid _ _ Hval2 Halltup2)).
-  rewrite iter_flet_val, fbinop_rep, bool_of_binop_impl, simpl_all_dec.
-  intros Hconstrs.
-  (*Might need lemma about equality of fmlas*)
-  assert (Hval3: valid_formula sigma (Fpred p (fst (get_indprop_args (alpha_f f))) (snd (get_indprop_args (alpha_f f))))). {
-    rewrite <- ind_form_decomp; auto.
-    inversion Hval2; subst; auto.
-  }
-  rewrite fmla_rewrite with(Hval2:=Hval3); [|apply ind_form_decomp; auto].
-  rewrite fpred_rep, Hindpred.
-  (*Now we can unfold the definition of [indpred_rep_single]*)
-  unfold indpred_rep_single.
-  rewrite simpl_all_dec; intros P Hallconstrs.
-  (*Now, we need to know that this constructor (f) is true
-    under p->P interp*)
-  assert (Hformf: formula_rep gamma_valid pd 
-    all_unif vt (interp_with_P pf p P) vv f Hvalf). {
-      rewrite <- prove_iter_and in Hallconstrs.
-      apply Hallconstrs.
-      rewrite in_map_iff. exists (formula_rep gamma_valid pd 
-        all_unif vt (interp_with_P pf p P) vv f Hvalf).
-      split; auto.
-      assert (Hex:=(in_dep_map (formula_rep gamma_valid pd  all_unif vt (interp_with_P pf p P) vv) _ Hform _ Hinf)).
-      destruct Hex as [Hval4 Hinf'].
-      erewrite fmla_rep_irrel. apply Hinf'.
-  }
-  (*Now we repeat the process again (alpha, [indpred_transform, etc])*)
-  revert Hformf.
-  rewrite alpha_f_equiv, indpred_decomp_equiv; auto.
-  unfold indpred_transform.
-  rewrite fmla_rep_irrel with
-    (Hval2:= (fforalls_valid _ _ Hval1 Halltup1)).
-  rewrite fforalls_val, simpl_all_dec.
-  intros. specialize (Hformf h).
-  revert Hformf.
-  rewrite (fmla_rep_irrel) with(Hval2:=(iter_flet_valid _ _ Hval2 Halltup2)).
-  rewrite iter_flet_val, fbinop_rep, bool_of_binop_impl, simpl_all_dec.
-  rewrite fmla_rewrite with(f1:=(tup_4 _))(Hval2:=Hval3); [|apply ind_form_decomp; auto].
-  rewrite fpred_rep. simpl.
-  destruct (predsym_eq_dec p p); auto; try contradiction.
-  assert (e= eq_refl). apply UIP_dec. apply predsym_eq_dec.
-  rewrite H. intros.
-  (*Need this in multiple places*)
-  assert ((substi_multi_let (interp_with_P pf p P) vt
-    (substi_mult vt vv (tup_1 (indpred_decomp (alpha_f f))) h)
-    (tup_2 (indpred_decomp (alpha_f f))) Halltup2) =
-    (substi_multi_let pf vt
-     (substi_mult vt vv (tup_1 (indpred_decomp (alpha_f f))) h)
-     (tup_2 (indpred_decomp (alpha_f f))) Halltup2)). {
-      apply substi_mult_notin_eq with(ps:=[p]); simpl; auto.
-      - apply indpred_decomp_let_notin with(ps:=[p]); auto.
-      - intros p'. destruct (predsym_eq_dec p p'); auto; subst.
-        intros. exfalso. apply H. left; auto.
-  }
-  (*Now, we need to show that the arguments to P are actually the same
-    because these terms cannot involve P*)
-  (*Ugly but oh well*)
-  match goal with | H: _ -> is_true (P ?y ?z) |- is_true (P ?y ?a) => assert (z = a) end.
-  - apply get_arg_list_pred_eq.
-    rewrite Forall_forall. intros x Hinx ty Hty1 Hty2.
-    rewrite H0.
-    rewrite term_rep_irrel with(Hty2:=Hty2).
-    apply term_predsym_agree; auto.
-    intros p' Hinp'.
-    unfold interp_with_P; simpl.
-    destruct (predsym_eq_dec p p'); subst; auto.
-    exfalso.
-    (*Use fact that p' not in x*)
-    assert (Hindt: ind_positive [p'] (tup_4 (indpred_decomp (alpha_f f)))).
-      apply indpred_decomp_last_pos; auto.
-    rewrite ind_form_decomp with(p:=p') in Hindt; auto.
-    inversion Hindt; subst.
-    specialize (H4 p' x Hinx H2).
-    rewrite Hinp' in H4. inversion H4.
-  - rewrite <- H1. apply Hformf.
-    clear H1 Hformf.
-    rewrite H0. clear H0.
-    (*TODO: need to prove that this valuation is the
-      same on all free vars of f' to get equivalence
-      Basically, know because everything in quants list + let
-      list is a bound variable and term is wf. But need to show*)
-    remember (substi_multi_let pf vt
-    (substi_mult vt vv (tup_1 (indpred_decomp (alpha_f f))) h)
-    (tup_2 (indpred_decomp (alpha_f f))) Halltup2) as vv'.
-    clear Heqvv'.
-    (*Now, we just need to prove that the [iter_and] of all of 
-      these constructors is true, when we interpre p with P
-      instead of [pf]. Here we will use the strict positivity
-      lemma TODO*)
-    rewrite iter_fand_rep.
-    rewrite iter_fand_rep in Hconstrs.
-    intros f' Hvalf' Hinf'.
-    specialize (Hconstrs f' Hvalf' Hinf').
-    revert Hconstrs.
-    eapply strict_pos_impred_implies_P with(ps:=[p])(Hform:=Hform); auto.
-    + left; auto.
-    + apply (indpred_decomp_and_strict_pos _ _ Hposa); auto.
-    + erewrite indpred_rep_single_val_eq; auto.
-      apply Hindpred.
-    + erewrite constrs_val_eq; auto. apply Hallconstrs.
-Qed.
-
-End Single.
-
-
-Lemma find_apply_pred_in (pf: pi_funpred gamma_valid pd)
-  (ps: list predsym)
-  (Ps: hlist
-  (fun p' : predsym =>
-   forall srts : list sort,
-   arg_list (domain (dom_aux pd)) (predsym_sigma_args p' srts) -> bool)
-  ps)
-  (p: predsym)
-  (Hinp: in_bool predsym_eq_dec p ps) :
-  find_apply_pred pf ps Ps p =
-  get_hlist_elt predsym_eq_dec Ps p Hinp.
-Proof.
-  induction ps; simpl.
-  - inversion Hinp.
-  - revert Hinp. simpl. 
-    destruct (predsym_eq_dec p a); subst; auto.
-Qed.
-
-Lemma find_apply_pred_notin (pf: pi_funpred gamma_valid pd)
-(ps: list predsym)
-(Ps: hlist
-(fun p' : predsym =>
- forall srts : list sort,
- arg_list (domain (dom_aux pd)) (predsym_sigma_args p' srts) -> bool)
-ps)
-(p: predsym) :
-~ In p ps ->
-find_apply_pred pf ps Ps p = preds gamma_valid pd pf p.
-Proof.
-  induction ps; simpl; auto.
-  intros Hnot. destruct (predsym_eq_dec p a); subst; auto.
-  exfalso. apply Hnot; auto.
-Qed.
-
-(*The least pred part for mutual recursion*)
-Theorem indpred_least_pred (pf: pi_funpred gamma_valid pd) 
-  (vt: val_typevar) (vv: val_vars pd vt)
-  (ps: list (predsym * list formula))
-  (Hform: Forall (Forall (valid_formula sigma)) (map snd ps)):
+  (ps: list (predsym * (list formula)))  
+  (f: formula)
+  (Hvalf: valid_formula sigma f)
+  (Hpos: ind_strictly_positive (map fst ps) f)
+  (Hform: Forall (Forall (valid_formula sigma)) (map snd ps))
+  (Hclosed: Forall (Forall closed_formula) (map snd ps))
+  (Hindpred: forall (p : predsym)
+    (Hinp : in_bool predsym_eq_dec p (map fst ps)),
+    preds gamma_valid pd pf p =
+    indpred_rep pf vt vv ps Hform p Hinp)
+  :
   forall (Ps: hlist
     (fun p' : predsym =>
     forall srts : list sort,
     arg_list (domain (dom_aux pd)) (predsym_sigma_args p' srts) -> bool)
     (map fst ps)),  
   (*If P holds of all of the constructors*)
-  (forall (fs : list formula) (Hform : Forall (valid_formula sigma) fs),
+  (forall (fs: list formula) (Hform: Forall (valid_formula sigma) fs), 
     In fs (map snd ps) ->
-      iter_and (map is_true (dep_map
-        (formula_rep gamma_valid pd all_unif vt
-        (interp_with_Ps pf (map fst ps) Ps) vv) fs Hform))) ->
-(*Then indpred_rep p fs x -> P x*)  
-  forall (p: predsym) (Hinp: in_bool predsym_eq_dec p (map fst ps))
-    (srts: list sort) 
-    (a: arg_list (domain (dom_aux pd)) 
-    (predsym_sigma_args p srts)),
-    indpred_rep pf vt vv ps Hform p Hinp srts a ->
-    get_hlist_elt predsym_eq_dec Ps p Hinp srts a.
-Proof.
-  intros Ps Hand p Hinp srts a.
-  unfold indpred_rep.
-  rewrite simpl_all_dec. intros.
-  apply H.
-  rewrite build_indpred_iff.
-  auto.
-Qed.
-
-Lemma strict_pos_impred_implies_P' (pf: pi_funpred gamma_valid pd) 
-(vt: val_typevar) (vv: val_vars pd vt)
-(ps: list (predsym * (list formula)))  
-(f: formula)
-(Hvalf: valid_formula sigma f)
-(Hpos: ind_strictly_positive (map fst ps) f)
-(Hform: Forall (Forall (valid_formula sigma)) (map snd ps))
-(Hclosed: Forall (Forall closed_formula) (map snd ps))
-(Hindpred: forall (p : predsym)
-  (Hinp : in_bool predsym_eq_dec p (map fst ps)),
-  preds gamma_valid pd pf p =
-  indpred_rep pf vt vv ps Hform p Hinp)
-:
-forall (Ps: hlist
-  (fun p' : predsym =>
-  forall srts : list sort,
-  arg_list (domain (dom_aux pd)) (predsym_sigma_args p' srts) -> bool)
-  (map fst ps)),  
-(*If P holds of all of the constructors*)
-(forall (fs: list formula) (Hform: Forall (valid_formula sigma) fs), 
-  In fs (map snd ps) ->
-iter_and (map is_true (dep_map
-  (formula_rep gamma_valid pd all_unif vt 
-    (interp_with_Ps pf (map fst ps) Ps) vv) fs Hform))) ->
-(*Then [[f]]_(p->indpred_rep p) implies [[f]]_(p->P)*) 
-formula_rep gamma_valid pd all_unif vt pf vv f Hvalf ->
-formula_rep gamma_valid pd all_unif vt (interp_with_Ps pf (map fst ps) Ps) vv f Hvalf.
+  iter_and (map is_true (dep_map
+    (formula_rep gamma_valid pd all_unif vt 
+      (interp_with_Ps pf (map fst ps) Ps) vv) fs Hform))) ->
+  (*Then [[f]]_(p->indpred_rep p) implies [[f]]_(p->P)*) 
+  formula_rep gamma_valid pd all_unif vt pf vv f Hvalf ->
+  formula_rep gamma_valid pd all_unif vt (interp_with_Ps pf (map fst ps) Ps) vv f Hvalf.
 Proof.
   intros Ps HandPs.
   generalize dependent vv.
@@ -2207,8 +1068,66 @@ Proof.
       * intros. apply H1; auto. right; auto.
 Qed.
 
-(*Now let's try mutual case*)
-Theorem indpred_constrs_true'
+(*We axiomatize alpha substitution, we will do it later*)
+Axiom alpha_f : formula -> formula.
+
+Axiom alpha_valid : forall (f: formula) (Hval: valid_formula sigma f),
+  valid_formula sigma (alpha_f f).
+
+Axiom alpha_f_equiv : forall (pf: pi_funpred gamma_valid pd)
+  (vt: val_typevar) (vv: val_vars pd vt) 
+  (f: formula) (Hvalf: valid_formula sigma f),
+  formula_rep gamma_valid pd all_unif vt pf vv f Hvalf =
+  formula_rep gamma_valid pd all_unif vt pf vv (alpha_f f) 
+    (alpha_valid f Hvalf).
+
+Axiom alpha_f_wf: forall (f: formula), fmla_wf (alpha_f f).
+
+Axiom alpha_valid_ind_form: forall (p: predsym) (f: formula),
+  valid_ind_form p f ->
+  valid_ind_form p (alpha_f f).
+
+Axiom alpha_pos: forall (ps: list predsym) (f: formula),
+  ind_positive ps f ->
+  ind_positive ps (alpha_f f).
+
+(*TODO: move*)
+(*If some pred P does not appear in any terms for [substi_multi_let],
+  then valuations are equal no matter what P is*)
+
+Lemma substi_mult_notin_eq (pf1 pf2: pi_funpred gamma_valid pd) 
+  (vt: val_typevar) (vv: val_vars pd vt) (l: list (vsymbol * term))
+  (ps: list predsym) Hall
+  (Hallnotin: Forall (fun x => (forall p, In p ps -> 
+    negb (predsym_in_term p (snd x)))) l) :
+  (forall p, ~ In p ps -> (preds gamma_valid pd pf1 p) = (preds gamma_valid pd pf2 p)) ->
+  (forall f, funs gamma_valid pd pf1 f = funs gamma_valid pd pf2 f) ->
+  substi_multi_let gamma_valid pd all_unif vt pf1 vv l Hall =
+  substi_multi_let gamma_valid pd all_unif vt pf2 vv l Hall.
+Proof.
+  revert Hall vv.
+  induction l; simpl; auto; intros.
+  inversion Hallnotin; subst.
+  destruct a.
+  assert (substi pd vt vv v
+  (term_rep gamma_valid pd all_unif vt pf1 vv t (snd v) (Forall_inv Hall)) =
+  (substi pd vt vv v
+     (term_rep gamma_valid pd all_unif vt pf2 vv t (snd v) (Forall_inv Hall)))). {
+    unfold substi. apply functional_extensionality_dep; intros; simpl.
+    destruct (vsymbol_eq_dec x v); subst; auto.
+    unfold eq_rec_r, eq_rec, eq_rect. simpl.
+    apply term_predsym_agree; auto.
+    intros p Hinp.
+    apply H. intro Hinp'.
+    simpl in H3. apply H3 in Hinp'.
+    rewrite Hinp in Hinp'. inversion Hinp'.
+  }
+  rewrite H1.
+  apply IHl; auto.
+Qed.
+
+(*Finally, we prove the main theorem*)
+Theorem indpred_constrs_true
   (pf: pi_funpred gamma_valid pd)
   (vt: val_typevar) (vv: val_vars pd vt)
   (indpred: list (predsym * list formula))
@@ -2323,11 +1242,11 @@ Proof.
   rewrite find_apply_pred_in with(Hinp:=Hinp').
   intros.
   (*Need this in multiple places*)
-  assert ((substi_multi_let (interp_with_Ps pf (map fst indpred) Ps) vt
-    (substi_mult vt vv (tup_1 (indpred_decomp (alpha_f f))) h)
+  assert ((substi_multi_let gamma_valid pd all_unif vt (interp_with_Ps pf (map fst indpred) Ps)
+    (substi_mult pd vt vv (tup_1 (indpred_decomp (alpha_f f))) h)
     (tup_2 (indpred_decomp (alpha_f f))) Halltup2) =
-    (substi_multi_let pf vt
-     (substi_mult vt vv (tup_1 (indpred_decomp (alpha_f f))) h)
+    (substi_multi_let gamma_valid pd all_unif vt pf
+     (substi_mult pd vt vv (tup_1 (indpred_decomp (alpha_f f))) h)
      (tup_2 (indpred_decomp (alpha_f f))) Halltup2)). {
       apply substi_mult_notin_eq with(ps:=map fst indpred); simpl; auto.
       - apply indpred_decomp_let_notin with(ps:=map fst indpred); auto.
@@ -2357,18 +1276,14 @@ Proof.
   - rewrite <- H0. apply Hformf.
     clear H0 Hformf.
     rewrite H. clear H.
-    (*TODO: need to prove that this valuation is the
-      same on all free vars of f' to get equivalence
-      Basically, know because everything in quants list + let
-      list is a bound variable and term is wf. But need to show*)
-    remember (substi_multi_let pf vt
-    (substi_mult vt vv (tup_1 (indpred_decomp (alpha_f f))) h)
+    remember (substi_multi_let gamma_valid pd all_unif vt pf
+    (substi_mult pd vt vv (tup_1 (indpred_decomp (alpha_f f))) h)
     (tup_2 (indpred_decomp (alpha_f f))) Halltup2) as vv'.
     clear Heqvv'.
     (*Now, we just need to prove that the [iter_and] of all of 
       these constructors is true, when we interpre p with P
       instead of [pf]. Here we will use the strict positivity
-      lemma TODO*)
+      lemma *)
     rewrite iter_fand_rep.
     rewrite iter_fand_rep in Hconstrs.
     intros f' Hvalf' Hinf'.
@@ -2383,8 +1298,13 @@ Proof.
       rewrite Forall_forall in Hclosed. apply Hclosed; auto.
 Qed.
 
-(*The non-mutually recursive version, proved from the stronger one*)
-Theorem indpred_constrs_true''
+End LeastPred.
+
+(*We prove simpler versions for the non-mutual case, since
+  working with hlists is awkward *)
+Section Single.
+
+Theorem indpred_constrs_true_single
   (pf: pi_funpred gamma_valid pd)
   (vt: val_typevar) (vv: val_vars pd vt)
   (p: predsym) (fs: list formula)
@@ -2399,7 +1319,7 @@ Theorem indpred_constrs_true''
     formula_rep gamma_valid pd all_unif vt pf vv f Hvalf).
 Proof.
   intros.
-  apply (indpred_constrs_true') with(indpred:=[(p, fs)])(Hform:=(Forall_single Hform));
+  apply (indpred_constrs_true) with(indpred:=[(p, fs)])(Hform:=(Forall_single Hform));
   simpl; auto.
   - intros p' Hinp'.
     assert (p = p'). { destruct (predsym_eq_dec p' p); subst; auto.
@@ -2415,95 +1335,32 @@ Proof.
   - rewrite app_nil_r. auto.
 Qed.
 
+Theorem indpred_least_pred_single (pf: pi_funpred gamma_valid pd) 
+  (vt: val_typevar) (vv: val_vars pd vt)
+  (p: predsym) (fs: list formula) (Hform: Forall (valid_formula sigma) fs):
+  forall (P:
+    forall srts : list sort,
+    arg_list (domain (dom_aux pd)) 
+      (predsym_sigma_args p srts) ->
+    bool
+  ),  
+  (*If P holds of all of the constructors*)
+  iter_and
+  (map is_true
+     (dep_map
+        (formula_rep gamma_valid pd 
+          all_unif vt (interp_with_P pf p P)  vv) fs Hform)) ->
+(*Then indpred_rep p fs x -> P x*)  
+  forall (srts : list sort)
+  (a: arg_list (domain (dom_aux pd)) 
+    (predsym_sigma_args p srts)),
+    indpred_rep_single pf vt vv p fs Hform srts a -> P srts a.
+Proof.
+  intros P Hand srts a. unfold indpred_rep_single.
+  rewrite simpl_all_dec. intros.
+  apply H. apply Hand.
+Qed.
+
+End Single.
 
 End IndPropRep.
-
-(*
-(*Now prove least fixpoint: For any other P 
-  such that all constructor formulas hold when p is
-  interpreted as P and for all x, indpred_rep x -> P x*)
-Lemma indpred_least_fp (v: valuation gamma_valid i) (p: predsym)
-(fs: list formula) (Hform: Forall (valid_formula sigma) fs) 
-(P: forall (srts: list sort),
-  arg_list (domain (dom_aux gamma_valid i)) 
-  (predsym_sigma_args p srts) -> bool):
-  iter_and (map is_true (dep_map (@formula_rep _ _
-    gamma_valid (interp_with_P i p P) 
-    all_unif (interp_P_val i p P v)) fs Hform)) ->
-  forall (srts: list sort) 
-  (a: arg_list (domain (dom_aux gamma_valid i)) 
-  (predsym_sigma_args p srts)),
-  indpred_rep v p fs Hform srts a -> P srts a.
-Proof.
-  intros Hand srts a. unfold indpred_rep; intros. apply H. apply Hand.
-Qed.
-
-(*Need to deal with mutually recursive inductive predicates*)
-
-(*Test: even and odd*)
-Unset Elimination Schemes.
-Inductive ev : nat -> Prop :=
-  | ev0': ev 0
-  | ev_odd: forall n, odd n -> ev (S n)
-with odd: nat -> Prop :=
-  | odd_ev: forall n, ev n -> odd (S n).
-Set Elimination Schemes.
-
-Scheme ev_ind := Minimality for ev Sort Prop
-with odd_ind := Minimality for odd Sort Prop.
-
-Check ev_ind.
-
-Set Bullet Behavior "Strict Subproofs".
-
-(*Prove equivalent first (just to see)*)
-Lemma ev_eq: forall n, 
-  (ev n <-> even n) /\
-  (odd n <-> ~ (even n)).
-Proof.
-  intros n. induction n using lt_wf_ind; simpl; split; intros; split; intros.
-  - destruct n; try constructor.
-    destruct n; inversion H0; subst; inversion H2; subst.
-    constructor. apply H; auto.
-  - destruct n; constructor. destruct n; inversion H0; subst.
-    constructor. apply H; auto.
-  - destruct n; inversion H0; subst.
-    destruct n; inversion H2; subst;
-    intro C; inversion C; subst.
-    assert (~ even n). apply H; auto. auto.
-  - destruct n. exfalso. apply H0; constructor.
-    constructor. destruct n; constructor.
-    apply H; auto. intro C.
-    apply H0. constructor; auto.
-Qed.
-
-(*Now give the predicate*)
-Definition test_ev: nat -> Prop :=
-  fun m => forall (P1 P2: nat -> Prop),
-    P1 0 ->
-    (forall n, P2 n -> P1 (S n)) ->
-    (forall n, P1 n -> P2 (S n)) ->
-    P1 m.
-
-Definition test_odd: nat -> Prop :=
-  fun m => forall (P1 P2: nat -> Prop),
-    P1 0 ->
-    (forall n, P2 n -> P1 (S n)) ->
-    (forall n, P1 n -> P2 (S n)) ->
-    P2 m.
-
-Lemma test_ev_correct: forall n,
-  ev n <-> test_ev n.
-Proof.
-  intros n. unfold test_ev; split; intros.
-  - apply (ev_ind) with(P:=P1) (P0:=P2); auto.
-  - specialize (H ev odd). apply H; constructor; auto.
-Qed.
-
-Lemma test_odd_correct: forall n,
-  odd n <-> test_odd n.
-Proof.
-  intros n. unfold test_odd; split; intros.
-  - apply odd_ind with(P:=P1)(P0:=P2); auto.
-  - specialize (H ev odd). apply H; constructor; auto.
-Qed.*)
